WIP

src/specs/Verify.ec
@@ -8,6 +8,7 @@ require import LoadVerificationKey.
 require import PrepareAggregatedCommitment.
 require import PrepareQueries.
 require import UInt256.
+require import Utils.
 require import Verifier.
 require import VerifyQuotientEvaluation.
 require import YulPrimops.
@@ -285,26 +286,6 @@ module Verify = {
    var _recursive_part_p1, _recursive_part_p2: g option;
     
    (* load verification key related *)
-   var vk_gate_setup_0X, vk_gate_setup_0Y,
-       vk_gate_setup_1X, vk_gate_setup_1Y,
-       vk_gate_setup_2X, vk_gate_setup_2Y,
-       vk_gate_setup_3X, vk_gate_setup_3Y,
-       vk_gate_setup_4X, vk_gate_setup_4Y,
-       vk_gate_setup_5X, vk_gate_setup_5Y,
-       vk_gate_setup_6X, vk_gate_setup_6Y,
-       vk_gate_setup_7X, vk_gate_setup_7Y : int;
-   var vk_gate_selectors_0X, vk_gate_selectors_1X, 
-       vk_gate_selectors_0Y, vk_gate_selectors_1Y: int;
-   var vk_permutation_0X, vk_permutation_0Y, 
-       vk_permutation_1X, vk_permutation_1Y, 
-       vk_permutation_2X, vk_permutation_2Y, 
-       vk_permutation_3X, vk_permutation_3Y: int;
-   var vk_lookup_table_0X, vk_lookup_table_0Y,
-       vk_lookup_table_1X, vk_lookup_table_1Y,
-       vk_lookup_table_2X, vk_lookup_table_2Y,
-       vk_lookup_table_3X, vk_lookup_table_3Y: int;
-   var vk_lookup_selector_X, vk_lookup_selector_Y: int;
-   var vk_lookup_table_type_X, vk_lookup_table_type_Y: int;
    var vk_recursive_flag: bool;
 
    (* initialize transcript *)
@@ -318,12 +299,10 @@ module Verify = {
    var verify_quotient_evaluation_opt;
 
    (* prepare queries *)
-   var prepare_queries_opt;
    var query_at_z_0, query_at_z_1, copy_permutation_first_aggregated_commitment_coeff, lookupSFirstAggregatedCommitment,
        lookupGrandProductFirstAggregatedCoefficient, query_t_poly_aggregated;
 
    (* prepare aggregated commitment *)
-   var prepare_aggregated_commitment_opt;
    var aggregatedAtZSlot, aggregatedOpeningAtZSlot, aggregatedAtZOmegaSlot, aggregatedOpeningAtZOmega, pairingPairWithGeneratorSlot, pairingBufferPointSlot;
    
    (* final pairing *)
@@ -331,54 +310,7 @@ module Verify = {
 
    var failed;
    failed <- false;
-
-    (* _loadVerificationKeys *)
-    vk_gate_setup_0X <- 8752182643819278825281358491109311747488397345835400146720638359015287854690;
-    vk_gate_setup_0Y <- 11702890106774794311109464320829961639285524182517416836480964755620593036625;
-    vk_gate_setup_1X <- 20333726085237242816528533108173405517277666887513325731527458638169740323846;
-    vk_gate_setup_1Y <- 20895759739260899082484353863151962651671811489085862903974918191239970565727;
-    vk_gate_setup_2X <- 1568732599965362807326380099663611053862348508639087822144187543479274466412;
-    vk_gate_setup_2Y <- 5821054758250780059685638301776364871013117602597489359484409980131967326794;
-    vk_gate_setup_3X <- 1869564366554527726271945732583360837778279311090061338642468249261166609475;
-    vk_gate_setup_3Y <- 6787073056745945161826226704190290609825180409911049644428579916838155209697;
-    vk_gate_setup_4X <- 457576930265342335264945522969406804501107665328727087867171094316559181535;
-    vk_gate_setup_4Y <- 15424863073888926344027107060444259361026863904290125685775015743583967752523;
-    vk_gate_setup_5X <- 17470132079837949645292768946901897910488674334073656384858846314172720305794;
-    vk_gate_setup_5Y <- 545412623592733862227844066395948813122937527333953380716629283051527996076;
-    vk_gate_setup_6X <- 3542620684081214281078362979824071457719243923292217179618867142734017714197;
-    vk_gate_setup_6Y <- 10380438707000372753007289103897630883671902212004026295360039945231108187502;
-    vk_gate_setup_7X <- 13086775255118926036233880981068687796723800497694631087151014741591951564618;
-    vk_gate_setup_7Y <- 97194583370920108185062801930585216368005987855712538133473341181290744675;
-    
-    vk_gate_selectors_0X <- 11090534100914016361232447120294745393211436081860550365760620284449885924457;
-    vk_gate_selectors_0Y <- 6190121082107679677011313308624936965782748053078710395209485205617091614781;
-    vk_gate_selectors_1X <- 15086136319636422536776088427553286399949509263897119922379735045147898875009;
-    vk_gate_selectors_1Y <- 14330561162787072568797012175184761164763459595199124517037991495673925464785;
-
-    vk_permutation_0X <- 21323538885080684424185174689480993185750201390966223018512354418490677522148;
-    vk_permutation_0Y <- 13825385863192118646834397710139923872086647553258488355179808994788744210563;
-    vk_permutation_1X <- 8390759602848414205412884900126185284679301543388803089358900543850868129488;
-    vk_permutation_1Y <- 7069161667387011886642940009688789554068768218554020114127791736575843662652;
-    vk_permutation_2X <- 21779692208264067614279093821878517213862501879831804234566704419708093761485;
-    vk_permutation_2Y <- 14513193766097634962386283396255157053671281137962954471134782133605379519908;
-    vk_permutation_3X <- 4751267043421347170875860608378639586591867931662910797110300384786346064625;
-    vk_permutation_3Y <- 11385717438670984215358012358002661303410243223751533068904005282628107986385;
-
-    vk_lookup_table_0X <- 20045313662746578028950791395157660351198208045597010788369662325700141348443;
-    vk_lookup_table_0Y <- 2200761695078532224145807378118591946349840073460005094399078719163643466856;
-    vk_lookup_table_1X <- 13866646217607640441607041956684111087071997201218815349460750486791109380780;
-    vk_lookup_table_1Y <- 13178446611795019678701878053235714968797421377761816259103804833273256298333;
-    vk_lookup_table_2X <- 5057503605752869531452842486824745179648819794307492731589448195268672785801;
-    vk_lookup_table_2Y <- 8597434312520299647191152876265164941580478223412397470356037586993894367875;
-    vk_lookup_table_3X <- 1342318055425277544055386589364579054544440640110901993487861472578322387903;
-    vk_lookup_table_3Y <- 4438354282468267034382897187461199764068502038746983055473062465446039509158;
-
-    vk_lookup_selector_X <- 21714794642552531775933093644480516421064284615960245486122726724547638127878;
-    vk_lookup_selector_Y <- 20374981665942106195451736226451722737514281476778224282304648903722926579601;
-
-    vk_lookup_table_type_X <- 196778531949039689886328474582670216324308721975620885373710029662715787742;
-    vk_lookup_table_type_Y <- 11005776646725047106517461026899305486268481542412200771754169232553006481646;
-    
+   
     vk_recursive_flag <- false;
     
     load_proof_opt <@ LoadProof.high(public_input_length_in_words, public_input, proof_length_in_words, state_poly_0, state_poly_1, state_poly_2, state_poly_3, copy_permutation_grand_product, lookup_s_poly, lookup_grand_product, quotient_poly_part_0, quotient_poly_part_1, quotient_poly_part_2, quotient_poly_part_3, state_poly_0_opening_at_z, state_poly_1_opening_at_z, state_poly_2_opening_at_z, state_poly_3_opening_at_z, state_poly_3_opening_at_z_omega, gate_selector_0_opening_at_z, copy_permutation_poly_0_opening_at_z, copy_permutation_poly_1_opening_at_z, copy_permutation_poly_2_opening_at_z, copy_permutation_grand_product_opening_at_z_omega, lookup_s_poly_opening_at_z_omega, lookup_grand_product_opening_at_z_omega, lookup_t_poly_opening_at_z, lookup_t_poly_opening_at_z_omega, lookup_selector_poly_opening_at_z, lookup_table_type_poly_opening_at_z, quotient_poly_opening_at_z, linearisation_poly_opening_at_z, opening_proof_at_z, opening_proof_at_z_omega, recursive_proof_length_in_words, vk_recursive_flag, recursive_part_p1, recursive_part_p2);
@@ -399,9 +331,7 @@ module Verify = {
 
     (query_at_z_0, query_at_z_1, copy_permutation_first_aggregated_commitment_coeff, lookupSFirstAggregatedCommitment, lookupGrandProductFirstAggregatedCoefficient, query_t_poly_aggregated) <@ PrepareQueries.high(state_z_in_domain, _quotient_poly_part_0, _quotient_poly_part_1, _quotient_poly_part_2, _quotient_poly_part_3, _state_poly_0_opening_at_z, _state_poly_1_opening_at_z, _state_poly_2_opening_at_z, _state_poly_3_opening_at_z, vk_lookup_table_0, vk_lookup_table_1, vk_lookup_table_2, vk_lookup_table_3, state_eta, vk_gate_setup_0, vk_gate_setup_1, vk_gate_setup_2, vk_gate_setup_3, vk_gate_setup_4, vk_gate_setup_5, vk_gate_setup_6, vk_gate_setup_7, _state_poly_3_opening_at_z_omega, state_v, state_z, _gate_selector_0_opening_at_z, state_alpha, alpha2, alpha3, alpha4, alpha5, alpha6, alpha7, alpha8, state_beta, state_gamma, vk_gate_selectors_1, vk_permutation_3, _copy_permutation_grand_product_opening_at_z_omega, l0_at_z, _copy_permutation_poly_0_opening_at_z, _copy_permutation_poly_1_opening_at_z, _copy_permutation_poly_2_opening_at_z, _lookup_grand_product_opening_at_z_omega, z_minus_last_omega, _lookup_t_poly_opening_at_z_omega, state_beta_lookup, _lookup_t_poly_opening_at_z, beta_gamma_plus_gamma, _lookup_table_type_poly_opening_at_z, _lookup_selector_poly_opening_at_z, state_gamma_lookup, beta_plus_one, ln_minus_one_at_z);
 
-    prepare_aggregated_commitment_opt <@ PrepareAggregatedCommitment.high_encapsulated(query_at_z_0, _quotient_poly_opening_at_z, query_at_z_1, state_v, _linearisation_poly_opening_at_z, _state_poly_0, _state_poly_0_opening_at_z, _state_poly_1, _state_poly_1_opening_at_z, _state_poly_2, _state_poly_2_opening_at_z, _state_poly_3_opening_at_z, (vk_gate_selectors_0X, vk_gate_selectors_0Y), _gate_selector_0_opening_at_z, (vk_permutation_0X, vk_permutation_0Y), _copy_permutation_poly_0_opening_at_z, (vk_permutation_1X, vk_permutation_1Y), _copy_permutation_poly_1_opening_at_z, (vk_permutation_2X, vk_permutation_2Y), _copy_permutation_poly_2_opening_at_z, _lookup_t_poly_opening_at_z, (vk_lookup_selector_X, vk_lookup_selector_Y), _lookup_selector_poly_opening_at_z, (vk_lookup_table_type_X, vk_lookup_table_type_Y), _lookup_table_type_poly_opening_at_z, copy_permutation_first_aggregated_commitment_coeff, state_u, _copy_permutation_grand_product, _copy_permutation_grand_product_opening_at_z_omega, _state_poly_3, _state_poly_3_opening_at_z_omega, _lookup_s_poly, _lookup_s_poly_opening_at_z_omega, lookupSFirstAggregatedCommitment, _lookup_grand_product, _lookup_grand_product_opening_at_z_omega, lookupGrandProductFirstAggregatedCoefficient, query_t_poly_aggregated, _lookup_t_poly_opening_at_z_omega);
-   failed <- failed \/ is_none prepare_aggregated_commitment_opt;
-   (aggregatedAtZSlot, aggregatedOpeningAtZSlot, aggregatedAtZOmegaSlot, aggregatedOpeningAtZOmega, pairingPairWithGeneratorSlot, pairingBufferPointSlot) <- oget prepare_aggregated_commitment_opt;
+    (aggregatedAtZSlot, aggregatedOpeningAtZSlot, aggregatedAtZOmegaSlot, aggregatedOpeningAtZOmega, pairingPairWithGeneratorSlot, pairingBufferPointSlot) <@ PrepareAggregatedCommitment.high_encapsulated(query_at_z_0, _quotient_poly_opening_at_z, query_at_z_1, state_v, _linearisation_poly_opening_at_z, _state_poly_0, _state_poly_0_opening_at_z, _state_poly_1, _state_poly_1_opening_at_z, _state_poly_2, _state_poly_2_opening_at_z, _state_poly_3_opening_at_z, vk_gate_selectors_0, _gate_selector_0_opening_at_z, vk_permutation_0, _copy_permutation_poly_0_opening_at_z, vk_permutation_1, _copy_permutation_poly_1_opening_at_z, vk_permutation_2, _copy_permutation_poly_2_opening_at_z, _lookup_t_poly_opening_at_z, vk_lookup_selector, _lookup_selector_poly_opening_at_z, vk_lookup_table_type, _lookup_table_type_poly_opening_at_z, copy_permutation_first_aggregated_commitment_coeff, state_u, _copy_permutation_grand_product, _copy_permutation_grand_product_opening_at_z_omega, _state_poly_3, _state_poly_3_opening_at_z_omega, _lookup_s_poly, _lookup_s_poly_opening_at_z_omega, lookupSFirstAggregatedCommitment, _lookup_grand_product, _lookup_grand_product_opening_at_z_omega, lookupGrandProductFirstAggregatedCoefficient, query_t_poly_aggregated, _lookup_t_poly_opening_at_z_omega);
 
   final_pairing_bool <@ FinalPairing.high(state_u, state_z, pairingPairWithGeneratorSlot, pairingBufferPointSlot, _opening_proof_at_z, _opening_proof_at_z_omega, vk_recursive_flag, recursive_part_p1, recursive_part_p2);
   failed <- failed \/ !final_pairing_bool;
@@ -678,3 +608,109 @@ rewrite load_store_same; by simplify.
 clear m1 m2 m3 m4 m5 m6 m7 m8 m9 m10 m11 m12 m13 m14 m15 m16 m17 m18 m19 
       m20 m21 m22 m23 m24 m25 m26 m27 m28 m29 m30 m31 m32 m33 m34 m35 m36 m37 m38 m39 m40 m41.
 *)
+
+lemma verify_mid_equiv_high_encapsulated:
+    equiv [
+      Verify.mid ~ Verify.high_encapsulated:
+        ={public_input_length_in_words} /\
+        public_input{1} = FieldR.asint public_input{2} /\
+        ={proof_length_in_words} /\
+        state_poly_0{1} = F_to_int_point(aspoint_G1 state_poly_0{2}) /\
+        state_poly_1{1} = F_to_int_point(aspoint_G1 state_poly_1{2}) /\
+        state_poly_2{1} = F_to_int_point(aspoint_G1 state_poly_2{2}) /\
+        state_poly_3{1} = F_to_int_point(aspoint_G1 state_poly_3{2}) /\
+        copy_permutation_grand_product{1} = F_to_int_point(aspoint_G1 copy_permutation_grand_product{2}) /\
+        lookup_s_poly{1} = F_to_int_point(aspoint_G1 lookup_s_poly{2}) /\
+        lookup_grand_product{1} = F_to_int_point(aspoint_G1 lookup_grand_product{2}) /\
+        quotient_poly_part_0{1} = F_to_int_point(aspoint_G1 quotient_poly_part_0{2}) /\
+        quotient_poly_part_1{1} = F_to_int_point(aspoint_G1 quotient_poly_part_1{2}) /\
+        quotient_poly_part_2{1} = F_to_int_point(aspoint_G1 quotient_poly_part_2{2}) /\
+        quotient_poly_part_3{1} = F_to_int_point(aspoint_G1 quotient_poly_part_3{2}) /\
+        state_poly_0_opening_at_z{1} = FieldR.asint state_poly_0_opening_at_z{2} /\
+        state_poly_1_opening_at_z{1} = FieldR.asint state_poly_1_opening_at_z{2} /\
+        state_poly_2_opening_at_z{1} = FieldR.asint state_poly_2_opening_at_z{2} /\
+        state_poly_3_opening_at_z{1} = FieldR.asint state_poly_3_opening_at_z{2} /\
+        state_poly_3_opening_at_z_omega{1} = FieldR.asint state_poly_3_opening_at_z_omega{2} /\
+        gate_selector_0_opening_at_z{1} = FieldR.asint gate_selector_0_opening_at_z{2} /\
+        copy_permutation_poly_0_opening_at_z{1} = FieldR.asint copy_permutation_poly_0_opening_at_z{2} /\
+        copy_permutation_poly_1_opening_at_z{1} = FieldR.asint copy_permutation_poly_1_opening_at_z{2} /\
+        copy_permutation_poly_2_opening_at_z{1} = FieldR.asint copy_permutation_poly_2_opening_at_z{2} /\
+        copy_permutation_grand_product_opening_at_z_omega{1} = FieldR.asint copy_permutation_grand_product_opening_at_z_omega{2} /\
+        lookup_s_poly_opening_at_z_omega{1} = FieldR.asint lookup_s_poly_opening_at_z_omega{2} /\
+        lookup_grand_product_opening_at_z_omega{1} = FieldR.asint lookup_grand_product_opening_at_z_omega{2} /\
+        lookup_t_poly_opening_at_z{1} = FieldR.asint lookup_t_poly_opening_at_z{2} /\
+        lookup_t_poly_opening_at_z_omega{1} = FieldR.asint lookup_t_poly_opening_at_z_omega{2} /\
+        lookup_selector_poly_opening_at_z{1} = FieldR.asint lookup_selector_poly_opening_at_z{2} /\
+        lookup_table_type_poly_opening_at_z{1} = FieldR.asint lookup_table_type_poly_opening_at_z{2} /\
+        quotient_poly_opening_at_z{1} = FieldR.asint quotient_poly_opening_at_z{2} /\
+        linearisation_poly_opening_at_z{1} = FieldR.asint linearisation_poly_opening_at_z{2} /\
+        opening_proof_at_z{1} = F_to_int_point(aspoint_G1 opening_proof_at_z{2}) /\
+        opening_proof_at_z_omega{1} = F_to_int_point(aspoint_G1 opening_proof_at_z_omega{2}) /\
+        ={recursive_proof_length_in_words} /\
+        recursive_part_p1{1} = F_to_int_point(aspoint_G1 recursive_part_p1{2}) /\
+        recursive_part_p2{1} = F_to_int_point(aspoint_G1 recursive_part_p2{2}) ==> 
+        ={res}
+    ].
+    proof.
+      proc.
+      simplify.
+      sp.
+      seq 3 3: (
+        (failed{1} /\ failed{2}) \/
+        (!failed{1} /\ !failed{2} /\
+        _public_input{1} = FieldR.asint _public_input{2} /\
+        _state_poly_0{1} = F_to_int_point(aspoint_G1 _state_poly_0{2}) /\
+        _state_poly_1{1} = F_to_int_point(aspoint_G1 _state_poly_1{2}) /\
+        _state_poly_2{1} = F_to_int_point(aspoint_G1 _state_poly_2{2}) /\
+        _state_poly_3{1} = F_to_int_point(aspoint_G1 _state_poly_3{2}) /\
+        _copy_permutation_grand_product{1} = F_to_int_point(aspoint_G1 _copy_permutation_grand_product{2}) /\
+        _lookup_s_poly{1} = F_to_int_point(aspoint_G1 _lookup_s_poly{2}) /\
+        _lookup_grand_product{1} = F_to_int_point(aspoint_G1 _lookup_grand_product{2}) /\
+        _quotient_poly_part_0{1} = F_to_int_point(aspoint_G1 _quotient_poly_part_0{2}) /\
+        _quotient_poly_part_1{1} = F_to_int_point(aspoint_G1 _quotient_poly_part_1{2}) /\
+        _quotient_poly_part_2{1} = F_to_int_point(aspoint_G1 _quotient_poly_part_2{2}) /\
+        _quotient_poly_part_3{1} = F_to_int_point(aspoint_G1 _quotient_poly_part_3{2}) /\
+        _state_poly_0_opening_at_z{1} = FieldR.asint _state_poly_0_opening_at_z{2} /\
+        _state_poly_1_opening_at_z{1} = FieldR.asint _state_poly_1_opening_at_z{2} /\
+        _state_poly_2_opening_at_z{1} = FieldR.asint _state_poly_2_opening_at_z{2} /\
+        _state_poly_3_opening_at_z{1} = FieldR.asint _state_poly_3_opening_at_z{2} /\
+        _state_poly_3_opening_at_z_omega{1} = FieldR.asint _state_poly_3_opening_at_z_omega{2} /\
+        _gate_selector_0_opening_at_z{1} = FieldR.asint _gate_selector_0_opening_at_z{2} /\
+        _copy_permutation_poly_0_opening_at_z{1} = FieldR.asint _copy_permutation_poly_0_opening_at_z{2} /\
+        _copy_permutation_poly_1_opening_at_z{1} = FieldR.asint _copy_permutation_poly_1_opening_at_z{2} /\
+        _copy_permutation_poly_2_opening_at_z{1} = FieldR.asint _copy_permutation_poly_2_opening_at_z{2} /\
+        _copy_permutation_grand_product_opening_at_z_omega{1} = FieldR.asint _copy_permutation_grand_product_opening_at_z_omega{2} /\
+        _lookup_s_poly_opening_at_z_omega{1} = FieldR.asint _lookup_s_poly_opening_at_z_omega{2} /\
+        _lookup_grand_product_opening_at_z_omega{1} = FieldR.asint _lookup_grand_product_opening_at_z_omega{2} /\
+        _lookup_t_poly_opening_at_z_omega{1} = FieldR.asint _lookup_t_poly_opening_at_z_omega{2} /\
+        _lookup_selector_poly_opening_at_z{1} = FieldR.asint _lookup_selector_poly_opening_at_z{2} /\
+        _lookup_table_type_poly_opening_at_z{1} = FieldR.asint _lookup_table_type_poly_opening_at_z{2} /\
+        _quotient_poly_opening_at_z{1} = FieldR.asint _quotient_poly_opening_at_z{2} /\
+        _linearisation_poly_opening_at_z{1} = FieldR.asint _linearisation_poly_opening_at_z{2} /\
+        _opening_proof_at_z{1} = F_to_int_point(aspoint_G1 _opening_proof_at_z{2}) /\
+        _opening_proof_at_z_omega{1} = F_to_int_point(aspoint_G1 _opening_proof_at_z_omega{2}) /\
+        _recursive_part_p1{1} = (omap F_to_int_point (omap aspoint_G1 _recursive_part_p1{2})) /\
+        _recursive_part_p2{1} = (omap F_to_int_point (omap aspoint_G1 _recursive_part_p2{2}))
+      )).
+      wp.
+      call (loadProof_mid_equiv_high false). skip. rewrite /point_map.
+      have H_tuple: forall (p: g), ((aspoint_G1 p).`1, (aspoint_G1 p).`2) = aspoint_G1 p by smt ().
+      progress.
+      rewrite F_to_int_point_inzmod_1 F_to_int_point_inzmod_2. exact H_tuple.
+      rewrite F_to_int_point_inzmod_1 F_to_int_point_inzmod_2. exact H_tuple.
+      rewrite F_to_int_point_inzmod_1 F_to_int_point_inzmod_2. exact H_tuple.
+      rewrite F_to_int_point_inzmod_1 F_to_int_point_inzmod_2. exact H_tuple.
+      rewrite F_to_int_point_inzmod_1 F_to_int_point_inzmod_2. exact H_tuple.
+      rewrite F_to_int_point_inzmod_1 F_to_int_point_inzmod_2. exact H_tuple.
+      rewrite F_to_int_point_inzmod_1 F_to_int_point_inzmod_2. exact H_tuple.
+      rewrite F_to_int_point_inzmod_1 F_to_int_point_inzmod_2. exact H_tuple.
+      rewrite F_to_int_point_inzmod_1 F_to_int_point_inzmod_2. exact H_tuple.
+      rewrite F_to_int_point_inzmod_1 F_to_int_point_inzmod_2. exact H_tuple.
+      rewrite F_to_int_point_inzmod_1 F_to_int_point_inzmod_2. exact H_tuple.
+      rewrite F_to_int_point_inzmod_1 F_to_int_point_inzmod_2. exact H_tuple.
+      rewrite F_to_int_point_inzmod_1 F_to_int_point_inzmod_2. exact H_tuple.
+      rewrite F_to_int_point_inzmod_1 F_to_int_point_inzmod_2. exact H_tuple.
+      rewrite F_to_int_point_inzmod_1 F_to_int_point_inzmod_2. exact H_tuple.
+      case H14. by progress. progress.
+      rewrite -H15 /F_to_int_point. print FieldQ.inFK.
+      (* replace point_map with F_to_int_point in loadProof mid to high *)      
